Merged old master and dev-gokul branch

list.dfy
@@ -67,32 +67,42 @@ method list_add_tail(new_node: Node, head: Node)
   internal_list_add(new_node, head.prev, head);
 }
 
+ghost predicate same_linked_list(nodes: seq<Node>)
+requires |nodes| >= 1 
+reads multiset(nodes)
+{
+  var ghost_nodes := nodes[0].nodes;
+  forall node' :: node' in nodes ==> node'.nodes == ghost_nodes
+}
+
 method internal_list_del(prev: Node, next: Node)
-  requires Valid(prev) && Valid(next) && Valid(prev.next)
+  requires Valid(prev) && Valid(next)
   requires prev.next.next == next
   requires prev != prev.next && prev.next != next
-  requires prev.nodes == next.nodes == prev.next.nodes
+  requires same_linked_list([prev, next])
   modifies prev, next, prev.next, multiset(prev.nodes)
   ensures Valid(prev)
   ensures Valid(next)
-  ensures prev.next == next
-  ensures next.prev == prev
-  ensures prev.nodes == next.nodes
-  ensures |prev.nodes| == |old(prev.nodes)| - 1
-  ensures old(prev.next) !in prev.nodes && old(next.prev) !in next.nodes
-  // ensures multiset(prev.nodes) == multiset(old(prev.nodes)) - multiset{old(prev.next)}
+  ensures same_linked_list([prev, next])
+  ensures (
+    var idx := IndexOf(old(prev.nodes), prev);
+    && (idx == |old(prev.nodes)| - 1 ==> prev.nodes == old(prev.nodes[1..])) // prev is last, removed val is first index
+    && (idx == |old(prev.nodes)| - 2 ==> prev.nodes == old(prev.nodes[..|prev.nodes|-1])) // prev is second last, removed is the last element
+    && (0 <= idx < |old(prev.nodes)|-2 ==> prev.nodes == old(prev.nodes[..idx+1])+old(prev.nodes[idx+2..])) // anything else, then join arr till prev_idx] + [prev_idx+2..]
+  )
 {
+  ghost var prev_idx := IndexOf(prev.nodes, prev);
+  ghost var next_idx := IndexOf(prev.nodes, next);
+  ghost var len := |prev.nodes|;
+
   var prev_next := prev.next; // maintain reference to removed node
   next.prev := prev;
   prev.next := next;
 
-  ghost var prev_idx := IndexOf(prev.nodes, prev);
-  ghost var removed_idx := IndexOf(prev.nodes, prev_next);
-  ghost var next_idx := IndexOf(prev.nodes, next);
-
   // 3 cases - prev is the last node, the second last node, or any other node
   // in each assert the position of prev_next and next, then proceed to remove prev_next from the list
-  if prev_idx == |prev.nodes| - 1 {
+
+  if prev_idx == len - 1 {
     assert prev.nodes[0] == prev_next;
     assert prev.nodes[1] == next;
 
@@ -102,7 +112,9 @@ method internal_list_del(prev: Node, next: Node)
       a'.nodes := new_nodes;
     }
     assert prev.nodes[0] == next;
-  } else if prev_idx == |prev.nodes| - 2 {
+  } else if prev_idx == len - 2 {
+    assert prev_idx != |prev.nodes|-1; 
+    assert prev_idx != |prev.nodes|-1;
     assert prev.nodes[0] == next;
     assert prev.nodes[|prev.nodes|-1] == prev_next;
 
@@ -111,6 +123,7 @@ method internal_list_del(prev: Node, next: Node)
       a'.nodes := new_nodes;
     }
   } else {
+    assert 0 <= prev_idx < |prev.nodes|-2; 
     assert prev.nodes[prev_idx+1] == prev_next;
     assert prev.nodes[prev_idx+2] == next;
     assert next_idx == prev_idx+2;
@@ -126,28 +139,29 @@ method internal_list_del(prev: Node, next: Node)
   }
 }
 
-// method list_del_entry(entry: Node)
-// requires Valid(entry) && Valid(entry.prev) && Valid(entry.next) 
-// requires entry != entry.prev && entry != entry.next
-// requires entry.next.nodes == entry.prev.nodes == entry.nodes
-// modifies entry, entry.prev, entry.next, multiset(entry.nodes), multiset(entry.prev.nodes)
-// ensures Valid(entry.prev)
-// ensures Valid(entry.next)
-// {
-//   var entry_next := entry.next;
-//   var entry_prev := entry.prev;
 
-//   // assert entry != entry.prev && entry != entry.next  ==> |entry.nodes| >= 2;
-//   assert entry.nodes[get_prev_seq_idx(entry.nodes, IndexOf(entry.nodes, entry))] == entry.prev;
-//   assert entry.nodes[get_next_seq_idx(entry.nodes, IndexOf(entry.nodes, entry))] == entry.next;
+method list_del_entry(entry: Node)
+requires Valid(entry) && Valid(entry.prev) && Valid(entry.next) 
+requires entry != entry.prev && entry != entry.next
+requires entry.next.nodes == entry.prev.nodes == entry.nodes
+modifies entry, entry.prev, entry.next, multiset(entry.nodes), multiset(entry.prev.nodes)
+ensures Valid(entry.prev)
+ensures Valid(entry.next)
+{
+  var entry_next := entry.next;
+  var entry_prev := entry.prev;
+
+  // assert entry != entry.prev && entry != entry.next  ==> |entry.nodes| >= 2;
+  assert entry.nodes[get_prev_seq_idx(entry.nodes, IndexOf(entry.nodes, entry))] == entry.prev;
+  assert entry.nodes[get_next_seq_idx(entry.nodes, IndexOf(entry.nodes, entry))] == entry.next;
   
-//   assert Valid(entry) && entry != entry.prev ==> |entry.nodes| >= 2;
-//   // assert Valid(entry.prev) && Valid(entry) && entry.nodes == entry.prev.nodes ==> entry.prev.next == entry;
-//   // assert Valid(entry.next) && Valid(entry) && entry.nodes == entry.next.nodes ==> entry.next.prev == entry;
-//   // assert entry.prev.next.next == entry.next;
-//   // assert entry.next.prev.prev == entry.prev;
+  assert Valid(entry) && entry != entry.prev ==> |entry.nodes| >= 2;
+  // assert Valid(entry.prev) && Valid(entry) && entry.nodes == entry.prev.nodes ==> entry.prev.next == entry;
+  // assert Valid(entry.next) && Valid(entry) && entry.nodes == entry.next.nodes ==> entry.next.prev == entry;
+  // assert entry.prev.next.next == entry.next;
+  // assert entry.next.prev.prev == entry.prev;
 
-//   internal_list_del(entry.prev, entry.next); 
+  internal_list_del(entry.prev, entry.next); 
 
-//   assert |entry.prev.nodes| == |entry.nodes| - 1;
-// }
+  assert |entry.prev.nodes| == |entry.nodes| - 1;
+}
